compiler/compilerScript.sml
@@ -40,9 +40,9 @@ val compile_def = Define`
     | NONE => Failure ParseError
     | SOME prog =>
        case infertype_prog c.inferencer_config (prelude ++ prog) init_infer_state of
-       | (Failure (Exc (locs, msg)), st) =>
+       | Failure (Exc (locs, msg)) =>
            Failure (TypeError (concat [msg; implode " at "; locs_to_string locs]))
-       | (Success ic, st) =>
+       | Success ic =>
           case backend$compile c.backend_config (prelude ++ prog) of
           | NONE => Failure CompileError
           | SOME (bytes,limit) => Success (bytes,limit)`;
@@ -52,8 +52,8 @@ val compile_explorer_def = Define`
     case parse_prog (lexer_fun input) of
     | NONE => Failure ParseError
     | SOME prog =>
-       case infertype_prog c.inferencer_config (prelude ++ prog) of
-       | Failure (locs, msg) => Failure (TypeError (concat [msg; implode " at "; locs_to_string locs]))
+       case infertype_prog c.inferencer_config (prelude ++ prog) init_infer_state of
+       | Failure (Exc (locs, msg)) => Failure (TypeError (concat [msg; implode " at "; locs_to_string locs]))
        | Success ic => Success (backend$compile_explorer c.backend_config (prelude ++ prog))`
 
 (* The top-level compiler *)
