compiler/inference/inferScript.sml
@@ -2,14 +2,9 @@ open preamble miscTheory astTheory namespaceTheory typeSystemTheory;
 open namespacePropsTheory;
 open infer_tTheory unifyTheory;
 open stringTheory ;
-
-(* Provisional: *)
-open ml_translatorLib;
-(****************)
-
 open ml_monadBaseTheory ml_monadBaseLib;
 
-val _ = new_theory "infer";
+Val _ = New_theory "infer";
 (* val _ = ParseExtras.temp_loose_equality(); *)
 val _ = monadsyntax.temp_add_monadsyntax()
 val _ = patternMatchesLib.ENABLE_PMATCH_CASES();
@@ -56,7 +51,7 @@ val lookup_st_ex_def = Define `
     | SOME v => return v`;
 
 val fresh_uvar_def = Define `
-(fresh_uvar : (infer_st, infer_t, infer_exn) M) =
+(fresh_uvar () : (infer_st, infer_t, infer_exn) M) =
   do uvar <- get_next_uvar;
      set_next_uvar (uvar + 1);
      return (Infer_Tuvar uvar)
@@ -67,7 +62,7 @@ n_fresh_uvar (n:num) =
   if n = 0 then
     return []
   else
-    do v <- fresh_uvar;
+    do v <- fresh_uvar ();
        vs <- n_fresh_uvar (n - 1);
        return (v::vs)
     od`;
@@ -75,9 +70,8 @@ n_fresh_uvar (n:num) =
 val init_infer_state_def = Define `
   (init_infer_state : infer_st) = <| next_uvar := 0; subst := FEMPTY |>`;
 
-(* TODO: remove that from the definitions *)
 val init_state_def = Define `
-init_state =
+init_state () =
   do
       set_next_uvar 0;
       set_subst FEMPTY;
@@ -195,11 +189,11 @@ val infer_deBruijn_subst_def = tDefine "infer_deBruijn_subst" `
 
 val infer_p_def = tDefine "infer_p" `
 (infer_p l ienv (Pvar n) =
-  do t <- fresh_uvar;
+  do t <- fresh_uvar ();
      return (t, [(n,t)])
   od) ∧
 (infer_p l ienv Pany =
-  do t <- fresh_uvar;
+  do t <- fresh_uvar ();
      return (t, [])
   od) ∧
 (infer_p l ienv (Plit (IntLit i)) =
@@ -279,7 +273,7 @@ constrain_op l op ts =
           return (Infer_Tapp [] (TC_name (Short "bool")))
        od
    | (Opapp, [t1;t2]) =>
-       do uvar <- fresh_uvar;
+       do uvar <- fresh_uvar ();
           () <- add_constraint l t1 (Infer_Tapp [t2;uvar] TC_fn);
           return uvar
        od
@@ -289,7 +283,7 @@ constrain_op l op ts =
        od
    | (Opref, [t]) => return (Infer_Tapp [t] TC_ref)
    | (Opderef, [t]) =>
-       do uvar <- fresh_uvar;
+       do uvar <- fresh_uvar ();
           () <- add_constraint l t (Infer_Tapp [uvar] TC_ref);
           return uvar
        od
@@ -384,18 +378,18 @@ constrain_op l op ts =
           return (Infer_Tapp [] TC_string)
         od
    | (VfromList, [t]) =>
-       do uvar <- fresh_uvar;
+       do uvar <- fresh_uvar ();
           () <- add_constraint l t (Infer_Tapp [uvar] (TC_name (Short "list")));
           return (Infer_Tapp [uvar] TC_vector)
        od
    | (Vsub, [t1;t2]) =>
-       do uvar <- fresh_uvar;
+       do uvar <- fresh_uvar ();
           () <- add_constraint l t1 (Infer_Tapp [uvar] TC_vector);
           () <- add_constraint l t2 (Infer_Tapp [] TC_int);
           return uvar
        od
    | (Vlength, [t]) =>
-       do uvar <- fresh_uvar;
+       do uvar <- fresh_uvar ();
           () <- add_constraint l t (Infer_Tapp [uvar] TC_vector);
           return (Infer_Tapp [] TC_int)
        od
@@ -404,18 +398,18 @@ constrain_op l op ts =
           return (Infer_Tapp [t2] TC_array)
        od
    | (AallocEmpty, [t1]) =>
-       do uvar <- fresh_uvar;
+       do uvar <- fresh_uvar ();
           () <- add_constraint l t1 (Infer_Tapp [] TC_tup);
           return (Infer_Tapp [uvar] TC_array)
        od
    | (Asub, [t1;t2]) =>
-       do uvar <- fresh_uvar;
+       do uvar <- fresh_uvar ();
           () <- add_constraint l t1 (Infer_Tapp [uvar] TC_array);
           () <- add_constraint l t2 (Infer_Tapp [] TC_int);
           return uvar
        od
    | (Alength, [t]) =>
-       do uvar <- fresh_uvar;
+       do uvar <- fresh_uvar ();
           () <- add_constraint l t (Infer_Tapp [uvar] TC_array);
           return (Infer_Tapp [] TC_int)
        od
@@ -444,7 +438,7 @@ val infer_e_def = tDefine "infer_e" `
 (infer_e l ienv (Raise e) =
   do t2 <- infer_e l ienv e;
      () <- add_constraint l t2 (Infer_Tapp [] TC_exn);
-     t1 <- fresh_uvar;
+     t1 <- fresh_uvar ();
      return t1
   od) ∧
 (infer_e l ienv (Handle e pes) =
@@ -488,7 +482,7 @@ val infer_e_def = tDefine "infer_e" `
           return (Infer_Tapp ts' (tid_exn_to_tc tn))
        od) ∧
 (infer_e l ienv (Fun x e) =
-  do t1 <- fresh_uvar;
+  do t1 <- fresh_uvar ();
      t2 <- infer_e l (ienv with inf_v := nsBind x (0,t1) ienv.inf_v) e;
      return (Infer_Tapp [t1;t2] TC_fn)
   od) ∧
@@ -517,7 +511,7 @@ val infer_e_def = tDefine "infer_e" `
     failwith (l, (implode "Empty pattern match"))
   else
     do t1 <- infer_e l ienv e;
-       t2 <- fresh_uvar;
+       t2 <- fresh_uvar ();
        () <- infer_pes l ienv pes t1 t2;
        return t2
   od) ∧
@@ -589,7 +583,7 @@ val infer_e_def = tDefine "infer_e" `
   od) ∧
 (infer_funs l ienv [] = return []) ∧
 (infer_funs l ienv ((f, x, e)::funs) =
-  do uvar <- fresh_uvar;
+  do uvar <- fresh_uvar ();
      t <- infer_e l (ienv with inf_v := nsBind x (0,uvar) ienv.inf_v) e;
      ts <- infer_funs l ienv funs;
      return (Infer_Tapp [uvar;t] TC_fn::ts)
@@ -615,7 +609,7 @@ val empty_inf_decls = Define `
 
 val infer_d_def = Define `
 (infer_d mn idecls ienv (Dlet locs p e) =
-  do () <- init_state;
+  do () <- init_state();
      n <- get_next_uvar;
      t1 <- infer_e (SOME locs) ienv e;
      (t2,env') <- infer_p (SOME locs) ienv p;
@@ -631,7 +625,7 @@ val infer_d_def = Define `
   od) ∧
 (infer_d mn idecls ienv (Dletrec locs funs) =
   do () <- guard (ALL_DISTINCT (MAP FST funs)) (SOME locs) (implode "Duplicate function name");
-     () <- init_state;
+     () <- init_state();
      next <- get_next_uvar;
      uvars <- n_fresh_uvar (LENGTH funs);
      env' <- return (nsAppend (alist_to_ns (list$MAP2 (\(f,x,e) uvar. (f,(0,uvar))) funs uvars)) ienv.inf_v);
@@ -765,7 +759,7 @@ check_weak_decls decls_impl decls_spec ⇔
 (* val check_tscheme_inst_def = Define `
   check_tscheme_inst _ (tvs_spec, t_spec) (tvs_impl, t_impl) ⇔
     let M =
-    do () <- init_state;
+    do () <- init_state();
        uvs <- n_fresh_uvar tvs_impl;
        t <- return (infer_deBruijn_subst uvs t_impl);
        () <- add_constraint NONE t_spec t
@@ -777,7 +771,7 @@ check_weak_decls decls_impl decls_spec ⇔
 
 val check_tscheme_inst_aux_def = Define `
   check_tscheme_inst_aux _ (tvs_spec, t_spec) (tvs_impl, t_impl) ⇔
-    do () <- init_state;
+    do () <- init_state();
        uvs <- n_fresh_uvar tvs_impl;
        t <- return (infer_deBruijn_subst uvs t_impl);
        () <- add_constraint NONE t_spec t
@@ -948,5 +942,6 @@ sub_completion tvs next_uvar s1 extra_constraints s2 =
   (pure_add_constraints s1 extra_constraints s2 ∧
    (count next_uvar SUBSET FDOM s2) ∧
    (!uv. uv ∈ FDOM s2 ⇒ check_t tvs {} (t_walkstar s2 (Infer_Tuvar uv))))`;
+
 
 val _ = export_theory ();
